\small

\begin{equation}
\dfrac{Dk}{Dt} = \nabla \cdot (\nu + \nu_{t} \bar{\sigma_{k}})\nabla k + P - \varepsilon
\end{equation}

\begin{equation}
\dfrac{D\epsilon}{Dt} = \nabla \cdot (\nu + \nu_{t} \bar{\sigma_{\epsilon}})\nabla \varepsilon + \dfrac{\hat{\varepsilon}}{k}(C_{\epsilon 1} P - C_{\epsilon 2} \varepsilon) 
\end{equation}

\begin{equation}
\begin{aligned}
\dfrac{D(\phi/k)}{Dt} = 
\bigg[ \nabla \cdot (\nu + \nu_{t} \bar{\sigma_{\phi}})\nabla (\phi/k) 
+ (2\nu) \nabla \textsurd k \cdot \nabla(\phi / k)/\textsurd k \bigg]
+ C_{p1} (2\alpha - 1) \dfrac{\hat{\varepsilon}}{k}(\phi/k) \\
+   C_{p2} \dfrac{P}{k}(\phi/k)  +   0.53 (1-\alpha) \dfrac{P}{k}(\phi/k) 
- \bigg[  (2\alpha - 1) \dfrac{\hat{\varepsilon}}{k}(\phi/k)  + (2\nu) \nabla \textsurd k \cdot \nabla(\phi / k)/\textsurd k \bigg]   \\
- (\phi/k) \dfrac{P}{k}
- (0.5 + 0.33\sigma_{\phi}) (\phi/k) (\nabla \phi^{1/2} \cdot \nabla \phi^{1/2}) k / \hat{\varepsilon}
+ C_{T}\sqrt{\dfrac{\nu_{t}}{\nu}} \dfrac{P}{k}
\end{aligned}
\end{equation}

\begin{equation}
\begin{aligned}
\dfrac{D(\psi/k)}{Dt} = \bigg[ \nabla \cdot (\nu + \nu_{t} \bar{\sigma_{\psi}})\nabla (\psi/k) 
+ (2\nu) \nabla \textsurd k \cdot \nabla(\psi / k)/\textsurd k \bigg] 
+ \bigg[ \dfrac{\phi}{k}\omega - \dfrac{P}{k}(\psi/k) \bigg] \\
+ \bigg[ C_{p2}\dfrac{P}{k}(\psi/k)  
- C_{p2}\dfrac{\phi}{k}\omega 
- 2.2 \alpha \dfrac{P}{k}(\psi/k) 
- C_{p1} \dfrac{\hat{\varepsilon}}{k} (1-\alpha) (\psi/k) \bigg] \\
+ \bigg[ C_{\mu}(2\alpha - 1)\dfrac{\phi}{k}\omega + (1-\alpha)\dfrac{\varepsilon}{k}(\psi/k) 
- (2\nu) \nabla \textsurd k \cdot \nabla(\psi / k)/\textsurd k \bigg]
+ C_{T}\sqrt{\dfrac{\nu_{t}}{\nu}}\omega \\
\end{aligned}
\end{equation}

\begin{equation*}
P =  \alpha \psi \cdot \omega + 0.4 (1-\alpha) 0.6 \alpha k |S|  + 0.6 (1-\alpha) \phi |S|
\end{equation*}
\begin{equation*}
\hat{\varepsilon} = \varepsilon / (1 + \beta_{k} \nu \dfrac{ \lvert \nabla k \rvert }{ \phi \sqrt{k} } )
\end{equation*}
\begin{equation*}
\nu_{t} = C_{\mu} \dfrac{\phi k}{\hat{\varepsilon}}  \hspace{2cm} \alpha = (1 + 1.5 \dfrac{\phi}{k})^{-1}
\end{equation*}


\vspace{1cm}

Where model constants are: 
\begin{equation*}
\bar{\sigma_{k}} = 1.2, \;\; \bar{\sigma_{\epsilon}} = 0.83 \;\; \bar{\sigma_{\phi}} = 0.4 \;\; \bar{\sigma_{\psi}} = 1.2
\end{equation*}
\begin{equation*}
C_{\mu} = 0.21, \;\;\;\; C_{p1} = 1.83,  \;\;\;\; C_{p2} = \dfrac{3}{5}, \;\;\;\; C_{p3} = 0.12
\end{equation*}
\begin{equation*}
C_{\epsilon 1} = 1.45, \;\; C_{\epsilon 2} = 1.83, \;\; C_{\epsilon 3} = 0.15, \;\;\;\;\;\; C_{pr} = 1.0, \;\;\;\;\;\; \beta_{k} = 0.09
\end{equation*}
\begin{equation*}
S = \dfrac{1}{2}(\nabla U + \nabla U^{T})
\end{equation*}


\normalsize

\cleardoublepage

\small

\begin{equation*}
k_{w} =  min(1,r^{+}/90) \dfrac{{u_{\tau}}^{2}}{{\beta_{k}}^{1/2}}
\end{equation*}

\begin{equation*}
\varepsilon_{w} =  \bigg(  0.229 {u_{\tau}}^{2} (5/r^{+})^{2}  + |\psi| \bigg) \dfrac{{u_{\tau}}^{2}}{\nu_{eff}}
\end{equation*}


\begin{equation*}
\phi_{w} =  f_{\phi r}(r^{+}) k_{w}
\end{equation*}


\begin{equation*}
\psi_{w} =  {\nu_{t}}_{w} \omega_{w}
\end{equation*}


\begin{equation*}
{\nu_{t}}_{w} = C_{\mu} \dfrac{{\phi}_{w} k_{w}}{\varepsilon_{w}}
\end{equation*}


\begin{equation*}
f_{\phi r}=
\begin{cases}
r^{+} < 5, \;\;\;\; 0\\
r^{+} > 5 \;\;and\;\; r^{+} < 45, \;\;\;\; 0.12 { \bigg( \dfrac{r^{+}}{45} \bigg) }^2 - 0.0014(1- (\dfrac{r^{+}}{45}))\\
r^{+} > 45 \;\;and\;\; r^{+} < 90, \;\;\;\; 0.015(r^{+} - 45)/45 + 0.12 \\
r^{+} > 90, \;\;\;\; 0.135
\end{cases}
\end{equation*}

